


$$y = \sum_{n=0}^{\infty} a_n x^n$$

$$(1+x^2) \sum_{n=0}^{\infty} (n+1)(n+2) a_{n+2} x^n - 2 \sum_{n=0}^{\infty} a_n x^n = 0$$

$$\sum_{n=0}^{\infty} \left((n+1)(n+2) a_{n+2} - 2a_n + (n-1)n a_n \right) x^n = 0$$

$$a_{n+2} = -\frac{(n-2)(n+1)}{(n+1)(n+2)} a_n$$

for even $a_2 = \frac{2}{2} a_0 = a_0 \quad a_4 = 0 \dots a_{2k} = 0 \quad (k \geq 2)$

for odd $n = 2k-1 \quad a_{2k+1} = -\frac{2k-3}{2k+1} a_{2k-1} = -\frac{2k-3}{2k+1} \left(-\frac{2k-5}{2k-1} \left(-\frac{2k-7}{2k-3} \dots \frac{1}{3} a_1 \right) \right)$
 $= \frac{(-1)^{k-1}}{(2k-1)} a_1$

$$y = \sum_{n \text{ even}} a_n x^n + \sum_{n \text{ odd}} a_n x^n$$

$$= a_0 (1+x^2) + a_1 \left(x + \sum_{k=1}^{\infty} \frac{(-1)^{k-1}}{(2k-1)} x^{2k+1} \right)$$

$$= a_0 y_1 + a_1 y_2$$

1 b) $y_1(0) = 1 \quad y_2(0) = 0$
 $y_1'(0) = 0 \quad y_2'(0) = 1$

1 c) $\frac{1}{1+x^2} = \sum_{n=0}^{\infty} (-1)^n x^{2n} = \sum_{n=0}^{\infty} \frac{(-1)^n + 1}{2} x^n$

$$y = \sum_{n=0}^{\infty} c_n x^n$$

$$(1+x^2) \sum_{n=0}^{\infty} (n+1)(n+2) c_{n+2} x^n - 2 \sum_{n=0}^{\infty} c_n x^n = \sum_{n=0}^{\infty} \frac{(-1)^n + 1}{2} x^n$$

$$\sum_{n=0}^{\infty} \left((n+1)(n+2) c_{n+2} - 2c_n + \frac{(-1)^n + 1}{2} \right) x^n = 0$$

$$(n+1)(n+2)C_{n+2} + (n+1)(n-2)C_n = \frac{(-1)^{n+1}}{2}$$

for $n = 2k$

$$(2k+2)(2k+1)C_{2k+2} + (2k-2)(2k+1)C_{2k} = (-1)^k$$

$$b_{k+1} - b_k = \frac{(-1)^k k}{2(2k+1)}$$

(d) ① $p(x) = \int \frac{1}{y_1(x)} dx = \frac{x}{2(1+x^2)} + \frac{1}{2} \arctan x$

$$y_2(x) = \frac{x}{2} + \frac{1+x^2}{2} \arctan x$$

② $W(y_1, y_2) = 1$

$$y_p = -u_1 \int u_2 \frac{1}{(1+x^2)^2} dx + u_2 \int u_1 \frac{1}{(1+x^2)^2} dx$$

$$= \frac{1}{4} + \frac{x}{2} \arctan x + \frac{1+x^2}{4} (\arctan x)^2$$

to fit $y(0) = 0$ $y'(0) = 0$

$$y(x) = y_p - \frac{1}{4}(1+x^2) = \frac{x}{2} \arctan x + \frac{1+x^2}{4} (\arctan x)^2 - \frac{x^2}{4}$$

